online invariant proof: comments for send_ping_invariant

examples/Online_with_secrecy/DY.OnlineS.Invariants.Proofs.fst
@@ -12,9 +12,16 @@ open DY.OnlineS.Invariants
 
 #set-options "--fuel 0 --ifuel 1 --z3rlimit 25  --z3cliopt 'smt.qi.eager_threshold=100'"
 
-/// In this module,
-/// we show that every protocol step maintains the protocol invariants.
+/// In this module, we show that
+/// the three protocol steps (send_ping, receive_ping_and_send_ack, and receive_ack)
+/// maintain the protocol invariants.
+///
+/// For every step s we show a lemma of the form:
+/// trace_invariant tr ==> trace_invariant ( trace after step s )
 
+
+
+/// The invariant lemma for the first step `send_ping`
 
 val send_ping_invariant:
   alice:principal -> bob:principal -> keys_sid:state_id ->
@@ -26,23 +33,192 @@ val send_ping_invariant:
     let (_ , tr_out) = send_ping alice bob keys_sid tr in
     trace_invariant tr_out
   ))
+(* The proof works by showing that the trace invariant is maintained
+   by every traceful action in the step.
+   So we replicate the actions of the step and show trace_invariant after each.
+   
+   (Note that we are now in the "Lemma context",
+   so we have to unfold the monadic lets and composition.)
+*)
 let send_ping_invariant alice bob keys_sid  tr =
-  let (n_a, tr_rand) = mk_rand NoUsage (nonce_label alice bob) 32 tr in
+  (* The first action is generating the nonce n_a.
+  
+     Note that we can't use let* here since we are not in the traceful monad.
+     Thus, we have to pass the trace `tr` explicitly as last argument.
+     And we get back the new trace `tr_rand`.
+  *)
+  let (n_a, tr_rand) = gen_rand_labeled (nonce_label alice bob) tr in
+  (* That the trace invariant holds after this action,
+     can be shown automatically.
+
+    There is a corresponding lemma in `DY.Core.Trace.Manipulation`:
+    `mk_rand_trace_invariant`.
+    It comes with an SMT Pattern an hence is applied automatically.
+  *)
   assert(trace_invariant tr_rand);
 
+  // Defining the abstract message does not change the trace,
+  // so we don't have to show anything.
   let ping = Ping {p_alice = alice; p_n_a = n_a} in 
+
+  (* The call of `pk_enc_for` in the traceful + option monad 
+     has to be unfolded:
+     * We pass the current trace `tr_rand` as las argument
+     * We need to make a case distinction on the resulting option
+       and show trace_invariant in each case separately
+  *)
   match pk_enc_for alice bob keys_sid key_tag ping tr_rand with
-  | (None, _) -> ()
+  | (None, _) -> ( 
+      (* If encryption fails, the trace is not changed,
+         and hence the resulting trace after send_ping is tr_rand.
+         Since we already showed trace_invariant for tr_rand,
+         we don't have to show anything else in this case.
+
+        If you want to check this,
+        you can uncomment the next lines
+      *)
+      // let (_ , tr_out) = send_ping alice bob keys_sid tr in 
+      // assert(tr_out == tr_rand);
+      // assert(trace_invariant tr_out);
+      ()
+    )
   | (Some ping_encrypted, tr_enc) -> (
+      (* If encryption succeeds, we get a new trace `tr_enc`.
+         With the lemma `pk_enc_for_invariant` in `DY.Simplified`,
+         we have that trace_invariant holds for tr_enc.
+
+         Observe, that this lemma can be shown automatically.
+         Hence, we don't even have to call it here.
+      *)
       assert(trace_invariant tr_enc);
+
+      (* The next traceful action is sending the encrypted message.
+
+         Again, we have to pass the current trace `tr_enc` as last argument.
+
+      *)
       let (msg_ts, tr_msg) = send_msg ping_encrypted tr_enc in
-      serialize_wf_lemma message (is_knowable_by (nonce_label alice bob) tr_rand) ping;
-      bytes_invariant_pk_enc_for tr_rand alice bob keys_sid key_tag ping;
+      (* To show trace_invariant after sending the message (for `tr_msg`),
+         we look at the lemma `send_msg_invariant` in `DY.Core.Trace.Manipulation`
+         which looks very promising.
+         However, that lemma has an additional pre-condition requiring that
+         the message needs to be publishable.
+         (That corresponds to the intuition that everything on the trace 
+         is readable by the attacker.)
+
+         So to call this lemma, we have to show `is_publishable tr_enc ping_encrypted`.
+         Looking at `DY.Simplified`, we find the lemma `pk_enc_for_is_publishable`,
+         which gives a bunch of pre-conditions for the plaintext (serialized `ping`) 
+         under which the ciphertext `ping_encrypted` is publishable.
+         We show each of those pre-conditions.
+      *)
+          (* The first is `has_pki_invariant`.
+
+             It is a technical requirement on the protocol invariants 
+             which we are not explaining here.
+
+             In `DY.OnlineS.Invariants` we have the lemma `protocol_invariants_p_has_pki_invariant`
+             showing this requirement.
+          *)
+          assert(has_pki_invariant);
+
+          (* The next requirement for `pk_enc_for_is_publishable` is `bytes_invariant tr_enc (serialize ping)`.
+
+             TODO              
+          *)
+          serialize_wf_lemma message (is_knowable_by (nonce_label alice bob) tr_rand) ping;
+
+          (* The next two pre-conditions say
+             that the serialized ping should be readable by Alice and Bob.
+             (Ignore the `long_term_key_label` for now.)
+
+             TODO: they are resolved with the same serialize_wf_lemma
+          *)
+
+          (* Finally, we need to show the disjunction of
+             * the pkenc_pred holds for the serialized ping or
+             * the serialized ping is publishable
+
+             In our case, the first is true, i.e., the encryption prediate is satisfied.
+             The predicate requires that the nonce contained in the ping
+             has the label `nonce_label alice' bob'`, where
+             * alice' is the name in the first component of the ping and
+             * bob' is the participant whos key is used for encryption.
+
+             Since we generate the nonce n_a in the beginning of this step
+             with the label `nonce_label alice bob`,
+             put the same alice in the first component of the ping
+             and use the key of bob for encryption (in pk_enc_for),
+             we satisfy the predicate.
+          *)
+          assert(pkenc_pred.pred tr_rand (long_term_key_type_to_usage (LongTermPkEncKey key_tag) bob) (serialize message ping));
+      (* Now we showed all pre-conditions of `pk_enc_for_is_publishable`
+         and can call this lemma to show that ping_encrypted is publishable.
+
+         Together with the `send_msg_invariant` lemma, 
+         we then obtain that `tr_msg` satisfies tha trace invariant.
+      *)
+      pk_enc_for_is_publishable tr_rand alice bob keys_sid key_tag ping;
       assert(trace_invariant tr_msg);
+
+      (* The last traceful action in this step is starting a new session *)
       let st = SentPing {sp_bob = bob; sp_n_a = n_a} in
       let (sid, tr_sess) = start_new_session alice st tr_msg in
+      (* `start_new_session` is just calling `new_session_id` and then `set_state`.
+         So we have to check that both of those maintain the trace invariant.
+
+         For `new_session_id` we find the lemma 
+         `new_session_id_same_trace` in `DY.Core.Trace.Manipulation`
+         which says that the trace is not changed.
+         Hence it trivially maintains the trace invariant.
+         It comes with an SMT pattern, so it is applied automatically.
+
+         In the same file, we have the lemma `set_state_invariant`,
+         which gives an additional pre-condition 
+         for when the trace after the state was set satisfies the trace invariant.
+         This pre-condition is that the new state must satisfy the state predicate.
+
+         The state predicate for the SentPing state requires that
+         the nonce stored in the state has the label `nonce_label alice' bob'`, where
+         * alice' is the storing principal
+         * bob' is the name stored in the first component of the state
+
+         Similarly to above,
+         we generated the nonce wit the label `nonce_label alice bob` and
+         alice is storing the new state, and
+         bob is stored in the first component of the state.
+         So the state prediate is satisfied
+      *)
+      assert(state_predicate_p.pred tr_msg alice sid st);
+       (* With this, we have all pre-conditions of `set_state_invariant`.
+          Since that lemma comes with an SMT pattern,
+          it is applied automatically.
+       *)
       assert(trace_invariant tr_sess)
   )
+
+(* The above proof was very detailed.
+   In fact, most of the proof is done automatically by F*
+   and we can remove most of the asserts.
+
+   If we just keep the necessary calls to lemmas,
+   we end up with the following very short proof.
+*)
+val send_ping_invariant_short_version:
+  alice:principal -> bob:principal -> keys_sid:state_id ->
+  tr:trace ->
+  Lemma
+  ( requires trace_invariant tr
+  )
+  (ensures (
+    let (_ , tr_out) = send_ping alice bob keys_sid tr in
+    trace_invariant tr_out
+  ))
+let send_ping_invariant_short_version alice bob keys_sid  tr =
+  let (n_a, tr_rand) = gen_rand_labeled (nonce_label alice bob) tr in
+  let ping = Ping {p_alice = alice; p_n_a = n_a} in 
+  serialize_wf_lemma message (is_knowable_by (nonce_label alice bob) tr_rand) ping;
+  pk_enc_for_is_publishable tr_rand alice bob keys_sid key_tag ping
 
 val decode_ping_proof:
   tr:trace ->
